$$ a^m✖a^n=a^{m+n} $$
$$ a^m➗a^n =a^{m-n}$$
$$ (a^m)^n = a^{mn}$$
$$ a^{-m} = \frac{1}{a^m}$$
$$ a^n✖b^n=(ab)^n$$
$$a^0=1(a≠0) 因为a的0次，a➗(a,0除以0无意义$$
$$正确表达任何数的0次都是1，0的0次方无意义$$

1. $$(-x^3+2x^2-5)(2x^2-3x+1)$$
$$ =-2x^5-3x^4-x^3+4x^2-6x^3+2x^2-10x^2+15x-5$$
$$=-2x^5-3x^4-5x^3-4x^3+15x-5$$
     
2. $$(3x^2+2)(5x^4+2x^2+3)-(5x^4+x^2+3)(3x^2+3)$$
   $$=(3x^2+2)(5x^4+x^2+3)+(3x^2+2)(x^2)-(3x^2+3)(5x^2+x^2+3)$$
   $$=-5x^2-x^2-3+3x^4+2x^2$$
   $$=3x^4-3x^2-3$$
     
3. $$(5x^2-2x+1)(x^2-3x+2)$$
   $$=5x^4-15x^3+10x^2-2x^3+6x^2-4x+x^2-3x+2$$
   $$=5x^4-17x^3+17x^2-7x+2$$

4. $$(2x^2+3)(5x^4+3x^2+2)-(5x^4+x^2+2)(2x^2+5)$$
   $$=(2x^2+3)(2x^2)-2(5x^4+x^2+2)$$
   $$=-6x^4+5x^2-4$$

5. $$设(ax^3-x+6)(3x^2+5x+b)=6x^5+10x^4-7x^3+13x^2+32x-12,求a,b的值$$
   $$解: ∵x^5次项系数3a=6∴a=2$$
   $$∵长数项6b=-12所以b=-2$$

6. $$设(6x^3-x^2+a)(bx^2+5x+3)=-12x^5+32x^4+13x^3-7x^2+10x+6,求a,b的值 $$
   $$解：∵x^5项系数6b=-12 所以 b=-2$$
   $$∵常数项3a=6 ∴a =2 $$

7. $$(-5xy+4z)(-5xy-4z)$$
#### 根据$(a-b)(a+b)=a^2-b^2$公式
$$ 解(-5xy)^2-(4z)^2=25x^2y^2-16z^2$$

8. $$(\frac{3}{4}x-\frac{2}{3}y)^2$$
   #### 根据公式$$(a-b)^2=a^2-2ab+b^2$$
$$解：原式 = \frac{9}{16}x^2-xy+\frac{4}{9}y^2$$

9. $$(m+1)^2-5(m+1)(m-1)+2(m-1)^2$$
    $$= m^2+2m+1-5m^2+5+2m^2-4m+2$$
    $$=-2m^2-2m+8$$

10. $$(2m-3n)(3n-2m)$$
    $$=-(3n-2m)(3n-2m)=-(3n-2m)^2$$
    $$=-9n^2+12mn-4m^2$$

11. $$(a+b+c)(a+b-c)(a-b+c)(-a+b+c)$$
    $$= ((a+b)^2-c^2)(c^2-(a-b)^2)$$
    $$=(a+b)^2c^2-(a+b)^2(a-b)^2-c^4+(a-b)^2c^2$$
    $$= 2a^2c^2+2b^2c^2+(a^2-b^2)^2-c^4$$
    $$=a^4+b^4-c^4+2a^2c^2+2b^2c^2-2a^2b^2$$

12. $$a^2+b^2=(a+b)^2-2ab$$
13. $$ a^2+b^2=(a-b)^2+2ab$$
14. $$ (a+b)^2=(a-b)^2+4ab$$
15. $$(a-b)^2=(a+b)^2-4ab$$
16. $$若(x+n)(x-3)=x^2-mx-6,则m=?,n=?$$
    $$解:(x+n)(x-3)=x^2-(3-n)x-3n$$
    $$∴3n=6 n=2$$
    $$m=3-n 所以 m =1$$

17. $$m^2-8m +16= (m-4)^2$$
18. $$(a+b)^2-4ab=(a-b)^2,则M = -4ab$$
19. $$(a-b)^2=8,ab=1,则a^2+b^2=$$
    $$解：a^2-2ab+b^2=8∴a^2+b^2=8+2ab=10$$

20. $$(a+b)(a-b)+(a+b)^2-2a^2=a^2-b^2+a^2+b^2+2ab-2a^2=2ab$$
    $$∵a=3,b=\frac{1}{3}$$
    $$ 原式=2$$

21. $$x^2+2xy+y^2=(x+y)^2$$
    $$解:∵x=\sqrt{3}+1 y=\sqrt{3}-1$$
    $$ 原式=2^2=4$$


22. $$x^2-y^2=(x+y)(x-y)$$
23. $$解：x=\sqrt{3}+1 y=\sqrt{3}-1$$
    $$原式=2\sqrt{3}(-2)=-4\sqrt{3}$$

24. $$a^2b+ab^2=ab(a+b)=3✖2=6$$
25. $$ a^2+b^2=(a+b)^2-2ab=9-4=5$$
    
    